Allow precondition stability to depend on homedir
Needed to know that the pathname was a subdirectory of tid's homedir to
prove the precondition is stable. This required the FsSpec precondition
to refer to the home directory, although it need not know much about the
home directory protocol.

Finishes proof of complete file_get_attr spec.

src/ConcurrentFS.v
@@ -118,9 +118,9 @@ Section ConcurrentFS.
       end.
 
   Definition precondition_stable A T (fsspec: FsSpec A T) homes tid :=
-    forall a tree tree', fs_pre (fsspec a) tree ->
+    forall a tree tree', fs_pre (fsspec a) (homes tid) tree ->
                     homedir_rely tid homes tree tree' ->
-                    fs_pre (fsspec a) tree'.
+                    fs_pre (fsspec a) (homes tid) tree'.
 
   Hint Resolve fs_rep_hashmap_incr.
 
@@ -201,7 +201,7 @@ Section ConcurrentFS.
                     {| precondition :=
                          fs_inv(P, sigma, tree, homedirs) /\
                          local_l tid (Sigma.l sigma) = Unacquired /\
-                         fs_pre (fsspec a) tree /\
+                         fs_pre (fsspec a) (homedirs tid) tree /\
                          precondition_stable fsspec homedirs tid;
                        postcondition :=
                          fun sigma' r =>
@@ -395,7 +395,7 @@ Section ConcurrentFS.
                     {| precondition :=
                          fs_inv(P, sigma, tree, homedirs) /\
                          local_l tid (Sigma.l sigma) = Unacquired /\
-                         fs_pre (fsspec a) tree /\
+                         fs_pre (fsspec a) (homedirs tid) tree /\
                          precondition_stable fsspec homedirs tid /\
                          update = fs_dirup (fsspec a) /\
                          (forall r tree0,
@@ -533,7 +533,7 @@ Section ConcurrentFS.
                     {| precondition :=
                          fs_inv(P, sigma, tree, homedirs) /\
                          local_l tid (Sigma.l sigma) = Unacquired /\
-                         fs_pre (fsspec a) tree /\
+                         fs_pre (fsspec a) (homedirs tid) tree /\
                          precondition_stable fsspec homedirs tid /\
                          update = fs_dirup (fsspec a) /\
                          (forall r tree0,
@@ -577,7 +577,7 @@ Section ConcurrentFS.
                     {| precondition :=
                          fs_inv(P, sigma, tree, homedirs) /\
                          local_l tid (Sigma.l sigma) = Unacquired /\
-                         fs_pre (fsspec a) tree /\
+                         fs_pre (fsspec a) (homedirs tid) tree /\
                          (forall r tree, fs_dirup (fsspec a) r tree = tree) /\
                          precondition_stable fsspec homedirs tid;
                        postcondition :=
@@ -623,9 +623,49 @@ Section ConcurrentFS.
   Qed.
 
   (* translate all system calls for extraction *)
+  (* TODO: add real directory updates to modifying system calls (ie, those that
+  use [write_syscall]'s) *)
 
   Definition file_get_attr inum :=
     retry_readonly_syscall (fun mscs => file_get_attr (fsxp P) inum mscs).
+
+  Theorem file_get_attr_ok : forall tid inum,
+      cprog_spec G tid
+                 (fun '(tree, homedirs, pathname, f) sigma =>
+                    {| precondition :=
+                         fs_inv(P, sigma, tree, homedirs) /\
+                         local_l tid (Sigma.l sigma) = Unacquired /\
+                         find_subtree (homedirs tid ++ pathname) tree = Some (TreeFile inum f);
+                       postcondition :=
+                         fun sigma' r =>
+                           exists tree',
+                             fs_inv(P, sigma', tree', homedirs) /\
+                             homedir_rely tid homedirs tree tree' /\
+                             local_l tid (Sigma.l sigma') = Unacquired /\
+                             match r with
+                             | Done (attr, _) => attr = BFILE.BFAttr f
+                             | TryAgain => False
+                             | SyscallFailed => True
+                             end |})
+                 (file_get_attr inum).
+  Proof.
+    unfold file_get_attr; intros.
+    unfold cprog_spec; intros;
+      eapply cprog_ok_weaken;
+      [ monad_simpl; eapply retry_readonly_syscall_ok;
+        eauto using opt_file_get_attr_ok | ];
+      simplify; finish.
+    unfold precondition_stable; simplify; simpl.
+    eapply homedir_rely_preserves_subtrees; eauto.
+  Qed.
+
+  Definition file_set_attr inum attr :=
+    write_syscall (fun mscs => OptFS.file_set_attr (fsxp P) inum attr mscs)
+                  (fun _ tree => tree).
+
+  Definition create dnum name :=
+    write_syscall (fun mscs => OptFS.create (fsxp P) dnum name mscs)
+                  (fun _ tree => tree).
 
   Definition lookup dnum names :=
     retry_readonly_syscall (fun mscs => lookup (fsxp P) dnum names mscs).
@@ -633,22 +673,12 @@ Section ConcurrentFS.
   Definition read_fblock inum off :=
     retry_readonly_syscall (fun mscs => OptFS.read_fblock (fsxp P) inum off mscs).
 
-  (* TODO: add real directory updates to these modifying system calls *)
-
-  Definition file_set_attr inum attr :=
-    write_syscall (fun mscs => OptFS.file_set_attr (fsxp P) inum attr mscs)
-                  (fun _ tree => tree).
-
   Definition file_truncate inum sz :=
     write_syscall (fun mscs => OptFS.file_truncate (fsxp P) inum sz mscs)
                   (fun _ tree => tree).
 
   Definition update_fblock_d inum off b :=
     write_syscall (fun mscs => OptFS.update_fblock_d (fsxp P) inum off b mscs)
-                  (fun _ tree => tree).
-
-  Definition create dnum name :=
-    write_syscall (fun mscs => OptFS.create (fsxp P) dnum name mscs)
                   (fun _ tree => tree).
 
   Definition rename dnum srcpath srcname dstpath dstname :=
